src/program_logic/staged_invariant_init.v
@@ -74,25 +74,26 @@ Proof.
   }
 Qed.
 
-Lemma wpc0_staged_inv_cancel s k mj' mj E e Φ Φc Pc:
+Lemma wpc0_staged_inv_cancel s k mj' mj E1 E2 e Φ Φc Pc:
+  E1 ⊆ E2 →
   (mj' ≤ mj)%Qp →
-  staged_inv_cancel E mj' Pc -∗
-  wpc0 s k mj E e (λ v, staged_inv_cancel E mj' Pc -∗ Φ v) Φc -∗
-  wpc0 s k mj E e Φ (Φc ∗ Pc).
+  staged_inv_cancel E1 mj' Pc -∗
+  wpc0 s k mj E2 e (λ v, staged_inv_cancel E1 mj' Pc -∗ Φ v) Φc -∗
+  wpc0 s k mj E2 e Φ (Φc ∗ Pc).
 Proof.
-  iIntros (Hle_mj) "Hsc Hwp".
+  iIntros (Hsub Hle_mj) "Hsc Hwp".
   iDestruct "Hsc" as (mj0 Einv mj_ishare mj_ikeep γ γ' ?) "Hsc".
   iDestruct "Hsc" as (Hlt Hinf Hinvalid Heq_mj) "(Htok2&H&Hitok_ikeep&#Hpri_inv)".
-  iLöb as "IH" forall (e).
+  iLöb as "IH" forall (e E2 Hsub).
   rewrite ?wpc0_unfold. rewrite /wpc_pre.
   iSplit; last first.
   {
     iDestruct "Hwp" as "(_&Hwp)".
     iClear "IH".
-    iAssert (∃ E', ⌜ E' ⊆ E ⌝ ∧ pri_inv Einv (staged_inv_inner E' Einv mj0 mj_ishare γ γ' γstatus Pc))%I as "Hpri_inv'".
-    { iExists E. iSplit; eauto. }
-    iClear "Hpri_inv". iDestruct "Hpri_inv'" as (E' Hsub) "#Hpri_inv".
-    iLöb as "IH" forall (E' Einv mj0 mj_ikeep mj_ishare γ γ' γstatus Hsub Heq_mj Hle_mj Hinvalid Hinf Hlt) "Hpri_inv".
+    iAssert (∃ E', ⌜ E' ⊆ E1 ⌝ ∧ pri_inv Einv (staged_inv_inner E' Einv mj0 mj_ishare γ γ' γstatus Pc))%I as "Hpri_inv'".
+    { iExists E1. iSplit; eauto. }
+    iClear "Hpri_inv". iDestruct "Hpri_inv'" as (E' Hsub') "#Hpri_inv".
+    iLöb as "IH" forall (E' Einv mj0 mj_ikeep mj_ishare γ γ' γstatus Hsub' Heq_mj Hle_mj Hinvalid Hinf Hlt) "Hpri_inv".
     iIntros (g ns D κs) "Hg #HC".
     iDestruct (pri_inv_tok_disj with "[$]") as %[Hdisj|Hval]; last first.
     { exfalso. apply Qp_lt_nge in Hinvalid. revert Hval. rewrite frac_valid.
@@ -151,6 +152,7 @@ Proof.
       replace (⊤ ∖ D ∖ Einv) with (⊤ ∖ (Einv ∪ D)) by set_solver.
       iSpecialize ("HPcr" with "[$] [$]").
       iApply (step_fupd2N_inner_wand with "HPcr"); auto.
+      { set_solver. }
       iIntros "(Hg&HPr&HPc)".
       replace (⊤ ∖ (Einv ∪ D)) with (⊤ ∖ D ∖ Einv) by set_solver.
       iMod (pri_inv_tok_enable with "[$Hg //]") as "(Hitok&Hg)".
@@ -215,10 +217,11 @@ Proof.
   iModIntro. simpl. iMod "Hwp". iModIntro.
   iNext. iMod "Hwp". iModIntro. iApply (step_fupd2N_wand with "Hwp").
   iIntros "($&Hwp)".
-  iIntros. iMod ("Hwp" with "[//]") as "($&$&Hwpc&$&$)". iModIntro. iApply ("IH" with "[$] [$] [$]").
+  iIntros. iMod ("Hwp" with "[//]") as "($&$&Hwpc&$&$)". iModIntro.
+  iApply ("IH" with "[] [$] [$] [$]").
+  { iPureIntro. destruct (to_val); set_solver. }
   eauto.
 Qed.
-
 
 Lemma wpc_staged_inv_init s k E e Φ Φc P Pc:
   later_tok ∗
