src/program_logic/staged_invariant_use_idle.v
@@ -46,9 +46,9 @@ Implicit Types i : positive.
 Implicit Types N : namespace.
 Implicit Types P Q R : iProp Σ.
 
-Lemma wpc_staged_inv_aux k e E1' E1 mj mj_wp mj_ukeep Φ Φc P :
-  staged_value_inuse k e E1' E1 mj mj_wp mj_ukeep Φ Φc P -∗
-  wpc0 NotStuck k mj E1 e Φ Φc.
+Lemma wpc_staged_inv_aux k e E1' mj mj_wp mj_ukeep Φ Φc P :
+  staged_value_inuse k e E1' ⊤ mj mj_wp mj_ukeep Φ Φc P -∗
+  wpc0 NotStuck k mj ⊤ e Φ Φc.
 Proof.
   iIntros "Hsv".
   iLöb as "IH" forall (e).
@@ -230,7 +230,7 @@ Proof.
     }
     iFrame "HNC".
     iMod (saved_prop_alloc
-            (wpc0 NotStuck k mj_wp E1 e2
+            (wpc0 NotStuck k mj_wp ⊤ e2
               (λ v : val Λ, ∃ Qnew : iPropI Σ, Qnew ∗ □ (Qnew -∗ C ==∗ P) ∗ (staged_value E1' Qnew P -∗ Φc ∧ Φ v))
               (Φc ∗ P))%I) as (γprop_stored') "#Hsaved1''".
     iMod (saved_prop_alloc Φc) as (γprop_remainder') "#Hsaved2''".
@@ -285,16 +285,15 @@ Proof.
   }
 Qed.
 
-Lemma wpc_staged_inv k E1 E1' e Φ Φc Qs P :
+Lemma wpc_staged_inv k E1 e Φ Φc Qs P :
   to_val e = None →
-  E1 ⊆ E1' →
-  staged_value E1' Qs P ∗
+  staged_value ⊤ Qs P ∗
   (Φc ∧ (Qs -∗ WPC e @ NotStuck; k; E1 {{λ v, ∃ Qnew, Qnew ∗ □ (Qnew -∗ C ==∗ P) ∗
-                                       (staged_value E1' Qnew P -∗ Φc ∧ Φ v)}}
+                                       (staged_value ⊤ Qnew P -∗ Φc ∧ Φ v)}}
                                  {{ Φc ∗ P }}))
   ⊢ WPC e @ NotStuck; k; E1 {{ Φ }} {{ Φc }}.
 Proof.
-  iIntros (Hnval Hsub) "(Hstaged&Hwp)".
+  iIntros (Hnval) "(Hstaged&Hwp)".
   iDestruct "Hstaged" as (??????) "(Hown&Hownstat&#Hsaved1&#Hsaved2&Hltok&Hitok&Hinv)".
   iDestruct "Hinv" as (mj_wp_init mj_ishare Hlt) "#Hinv".
   rewrite /staged_inv.
@@ -432,8 +431,8 @@ Proof.
 
   iFrame "HNC".
   iMod (saved_prop_alloc
-          (wpc0 NotStuck k mj_wp E1 e2
-            (λ v : val Λ, ∃ Qnew : iPropI Σ, Qnew ∗ □ (Qnew -∗ C ==∗ P) ∗ (staged_value E1' Qnew P -∗ Φc ∧ Φ v))
+          (wpc0 NotStuck k mj_wp ⊤ e2
+            (λ v : val Λ, ∃ Qnew : iPropI Σ, Qnew ∗ □ (Qnew -∗ C ==∗ P) ∗ (staged_value ⊤ Qnew P -∗ Φc ∧ Φ v))
             (Φc ∗ P))%I) as (γprop_stored') "#Hsaved1''".
   iMod (saved_prop_alloc Φc) as (γprop_remainder') "#Hsaved2''".
   iMod (own_update_2 _ _ _ (● Excl' (γprop_stored', γprop_remainder') ⋅
@@ -481,7 +480,7 @@ Proof.
         etransitivity; first eapply Qp_le_min_l.
         eapply Qp_le_min_r.
   }
-  iAssert (staged_value_inuse k e2 E1' E1 mj mj_wp mj_ukeep Φ Φc P) with "[-]" as "Hsv".
+  iAssert (staged_value_inuse k e2 ⊤ ⊤ mj mj_wp mj_ukeep Φ Φc P) with "[-]" as "Hsv".
   {
     iExists _, _, mj_ishare, _, _, _, _, _. iExists _. iFrame "∗".
     iSplit; first eauto.
